Test.lean
@@ -1,2 +1,1 @@
 import Test.MIR
-import Test.Onchain
