Test/MIR.lean
@@ -1,7 +1,5 @@
 import Test.MIR.Helpers
-import Test.MIR.AnalysisUnit
-import Test.MIR.ANFUnit
 import Test.MIR.Golden
-import Test.MIR.OptimizeUnit
 import Test.MIR.OptimizeGolden
 import Test.MIR.LowerGolden
+import Test.MIR.Suites
